code/ecdsa/Hacl.Impl.EC.LowLevel.fsti
@@ -19,7 +19,7 @@ open Hacl.Impl.EC.Setup
 #set-options "--z3rlimit 100"
 
 
-val uploadZeroImpl: #c: curve -> f: felem c -> Stack unit 
+val uploadZeroImpl: #c: curve -> f: felem c -> Stack unit
   (requires fun h -> live h f)
   (ensures fun h0 _ h1 -> as_nat c h1 f == 0 /\ modifies (loc f) h0 h1)
 
@@ -27,162 +27,165 @@ val uploadOneImpl: #c: curve -> f: felem c -> Stack unit
   (requires fun h -> live h f)
   (ensures fun h0 _ h1 -> as_nat c h1 f == 1 /\ modifies (loc f) h0 h1)
 
-val uploadZeroPoint: #c: curve -> p: point c -> 
+val uploadZeroPoint: #c: curve -> p: point c ->
   Stack unit
   (requires fun h -> live h p)
   (ensures fun h0 _ h1 ->
-    let len = getCoordinateLenU64 c in 
+    let len = getCoordinateLenU64 c in
     modifies (loc p) h0 h1 /\
-    as_nat c h1 (gsub p (size 0) len) == 0 /\ 
+    as_nat c h1 (gsub p (size 0) len) == 0 /\
     as_nat c h1 (gsub p len len) == 0 /\
-    as_nat c h1 (gsub p (size 2 *! len) len) == 0) 
+    as_nat c h1 (gsub p (size 2 *! len) len) == 0)
 
-val add_bn: #c: curve -> x: felem c -> y: felem c -> result: felem c -> 
+val add_bn: #c: curve -> x: felem c -> y: felem c -> result: felem c ->
   Stack uint64
-    (requires fun h -> live h x /\ live h y /\ live h result /\ eq_or_disjoint x result /\ eq_or_disjoint y result)
-    (ensures fun h0 r h1 -> modifies (loc result) h0 h1 /\ v r <= 1 /\ 
-      as_nat c h1 result + v r * (pow2 (getPower c)) == as_nat c h0 x + as_nat c h0 y)   
+  (requires fun h -> live h x /\ live h y /\ live h result /\ eq_or_disjoint x result /\ eq_or_disjoint y result /\ eq_or_disjoint x y)
+  (ensures fun h0 r h1 -> modifies (loc result) h0 h1 /\ v r <= 1 /\
+    as_nat c h1 result + v r * (pow2 (getPower c)) == as_nat c h0 x + as_nat c h0 y)
 
-val add_long_bn: #c: curve -> x: widefelem c -> y: widefelem c -> result: widefelem c -> 
-  Stack uint64 
-  (requires fun h -> live h x /\ live h y /\ live h result /\ eq_or_disjoint x result /\ eq_or_disjoint y result)
-  (ensures fun h0 r h1 -> modifies (loc result) h0 h1 /\ v r <= 1 /\ 
+val add_long_bn: #c: curve -> x: widefelem c -> y: widefelem c -> result: widefelem c ->
+  Stack uint64
+  (requires fun h -> live h x /\ live h y /\ live h result /\ eq_or_disjoint x result /\ eq_or_disjoint y result /\ eq_or_disjoint x y)
+  (ensures fun h0 r h1 -> modifies (loc result) h0 h1 /\ v r <= 1 /\
     wide_as_nat c h1 result + v r * pow2 (getLongPower c) == wide_as_nat c h0 x + wide_as_nat c h0 y)
 
-val add_dep_prime: #c: curve -> x: felem c -> t: uint64 {uint_v t == 0 \/ uint_v t == 1} -> result: felem c -> 
-  Stack uint64
-  (requires fun h -> live h x /\ live h result /\ eq_or_disjoint x result)
-  (ensures fun h0 r h1 -> modifies (loc result) h0 h1 /\ v r <= 1 /\ (
-    if uint_v t = 1 then 
-      as_nat c h1 result + uint_v r * (pow2 (getPower c))  == as_nat c h0 x + getPrime c
-    else
-      as_nat c h1 result  == as_nat c h0 x))  
- 
 
-val sub_bn: #c: curve -> x: felem c -> y:felem c -> result: felem c -> 
+val sub_bn: #c: curve -> x: felem c -> y:felem c -> result: felem c ->
   Stack uint64
-  (requires fun h -> live h x /\ live h y /\ live h result /\ eq_or_disjoint x result /\ eq_or_disjoint y result)
-  (ensures fun h0 r h1 -> modifies1 result h0 h1 /\ v r <= 1 /\ 
+  (requires fun h -> live h x /\ live h y /\ live h result /\ eq_or_disjoint x result /\ eq_or_disjoint y result /\ eq_or_disjoint x y)
+  (ensures fun h0 r h1 -> modifies1 result h0 h1 /\ v r <= 1 /\
     as_nat c h1 result - v r * (pow2 (getPower c)) == as_nat c h0 x - as_nat c h0 y)
 
-val sub_bn_gl: #c: curve -> x: felem c -> y: glbuffer uint64 (getCoordinateLenU64 c) 
-  -> result: felem c -> 
+
+val sub_bn_order: #c: curve -> x: felem c -> result: felem c ->
   Stack uint64
-  (requires fun h -> live h x /\ live h y /\ live h result /\ disjoint x result /\ disjoint y result)
-  (ensures fun h0 r h1 -> modifies (loc result) h0 h1 /\ v r <= 1 /\ 
-    as_nat c h1 result - v r * (pow2 (getPower c)) == as_nat c h0 x  - as_nat_il c h0 y /\ (
-    if uint_v r = 0 then 
-      as_nat c h0 x >= as_nat_il c h0 y 
-    else 
-      as_nat c h0 x < as_nat_il c h0 y))
+  (requires fun h -> live h x /\ live h result /\ disjoint x result)
+  (ensures fun h0 r h1 -> modifies (loc result) h0 h1 /\ v r <= 1 /\
+    as_nat c h1 result - v r * (pow2 (getPower c)) == as_nat c h0 x - getOrder #c /\ (
+    if uint_v r = 0 then
+      as_nat c h0 x >= getOrder #c
+    else
+      as_nat c h0 x < getOrder #c))
+
+
+val sub_bn_prime: #c: curve -> x: felem c -> result: felem c ->
+  Stack uint64
+  (requires fun h -> live h x /\ live h result /\ disjoint x result)
+  (ensures fun h0 r h1 -> modifies (loc result) h0 h1 /\ v r <= 1 /\
+    as_nat c h1 result - v r * (pow2 (getPower c)) == as_nat c h0 x - getPrime c /\ (
+    if uint_v r = 0 then
+      as_nat c h0 x >= getPrime c
+    else
+      as_nat c h0 x < getPrime c))
+
 
 
 val short_mul_bn: #c: curve -> a: glbuffer uint64 (getCoordinateLenU64 c) -> b: uint64 -> result: widefelem c -> Stack unit
   (requires fun h -> live h a /\ live h result /\ wide_as_nat c h result = 0)
-  (ensures fun h0 _ h1 -> modifies (loc result) h0 h1 /\ 
-    as_nat_il c h0 a * uint_v b = wide_as_nat c h1 result /\ 
+  (ensures fun h0 _ h1 -> modifies (loc result) h0 h1 /\
+    as_nat_il c h0 a * uint_v b = wide_as_nat c h1 result /\
     wide_as_nat c h1 result < (pow2 (getPower c)) * pow2 64)
 
 
 val short_mul_prime: #c: curve -> b: uint64 -> result: widefelem c -> Stack unit
   (requires fun h -> live h result /\ wide_as_nat c h result = 0)
-  (ensures fun h0 _ h1 -> modifies (loc result) h0 h1 /\ 
-    getPrime c * uint_v b = wide_as_nat c h1 result /\ 
+  (ensures fun h0 _ h1 -> modifies (loc result) h0 h1 /\
+    getPrime c * uint_v b = wide_as_nat c h1 result /\
     wide_as_nat c h1 result < (pow2 (getPower c))  * pow2 64)
 
 
 val square_bn: #c: curve -> f: felem c -> out: widefelem c -> Stack unit
     (requires fun h -> live h out /\ live h f /\ eq_or_disjoint f out)
-    (ensures  fun h0 _ h1 -> modifies (loc out) h0 h1 /\ 
+    (ensures  fun h0 _ h1 -> modifies (loc out) h0 h1 /\
       wide_as_nat c h1 out = as_nat c h0 f * as_nat c h0 f)
-      
 
-val reduction_prime_2prime_with_carry: #c: curve -> x: widefelem c -> result: felem c -> 
-  Stack unit 
-    (requires fun h -> 
+
+val reduction_prime_2prime_with_carry: #c: curve -> x: widefelem c -> result: felem c ->
+  Stack unit
+    (requires fun h ->
       live h x /\ live h result /\ eq_or_disjoint x result /\ wide_as_nat c h x < 2 * getPrime c)
-    (ensures fun h0 _ h1 -> 
+    (ensures fun h0 _ h1 ->
       modifies (loc result) h0 h1 /\ as_nat c h1 result = wide_as_nat c h0 x % getPrime c)
 
 
-val reduction_prime_2prime: #c: curve -> x: felem c -> result: felem c -> 
+val reduction_prime_2prime: #c: curve -> x: felem c -> result: felem c ->
   Stack unit
-    (requires fun h -> 
+    (requires fun h ->
       live h x /\ live h result /\ eq_or_disjoint x result)
-    (ensures fun h0 _ h1 -> 
+    (ensures fun h0 _ h1 ->
       modifies (loc result) h0 h1 /\ as_nat c h1 result == as_nat c h0 x % getPrime c)
 
 let fromDomain #c a = fromDomain_ #c #DH a
 
 let toDomain #c a = toDomain_ #c #DH a
 
-val felem_add: #c: curve -> a: felem c -> b: felem c -> out: felem c -> 
+val felem_add: #c: curve -> a: felem c -> b: felem c -> out: felem c ->
   Stack unit
-    (requires (fun h0 -> 
+    (requires (fun h0 ->
       live h0 a /\ live h0 b /\ live h0 out /\ eq_or_disjoint a out /\ eq_or_disjoint b out /\
       as_nat c h0 a < getPrime c /\ as_nat c h0 b < getPrime c))
-    (ensures (fun h0 _ h1 -> 
-      modifies (loc out) h0 h1 /\ 
+    (ensures (fun h0 _ h1 ->
+      modifies (loc out) h0 h1 /\
       as_nat c h1 out == (as_nat c h0 a + as_nat c h0 b) % getPrime c /\
       as_nat c h1 out == toDomain #c((fromDomain #c (as_nat c h0 a) + fromDomain #c (as_nat c h0 b)) % getPrime c)))
 
 
-val felem_double: #c: curve -> a: felem c -> out: felem c -> 
-  Stack unit 
-    (requires (fun h0 -> 
+val felem_double: #c: curve -> a: felem c -> out: felem c ->
+  Stack unit
+    (requires (fun h0 ->
       live h0 a /\ live h0 out /\ eq_or_disjoint a out /\ as_nat c h0 a < getPrime c))
-    (ensures (fun h0 _ h1 -> 
-      modifies (loc out) h0 h1 /\ 
+    (ensures (fun h0 _ h1 ->
+      modifies (loc out) h0 h1 /\
       as_nat c h1 out == (2 * as_nat c h0 a) % getPrime c /\
       as_nat c h1 out == toDomain #c (2 * fromDomain #c (as_nat c h0 a) % getPrime c)))
 
 
-val felem_sub: #c: curve -> a: felem c -> b: felem c -> out: felem c -> 
-  Stack unit 
-  (requires (fun h0 -> 
+val felem_sub: #c: curve -> a: felem c -> b: felem c -> out: felem c ->
+  Stack unit
+  (requires (fun h0 ->
     live h0 out /\ live h0 a /\ live h0 b /\ eq_or_disjoint a out /\ eq_or_disjoint b out /\
     as_nat c h0 a < getPrime c /\ as_nat c h0 b < getPrime c))
-  (ensures (fun h0 _ h1 -> modifies (loc out) h0 h1 /\ 
+  (ensures (fun h0 _ h1 -> modifies (loc out) h0 h1 /\
     as_nat c h1 out == (as_nat c h0 a - as_nat c h0 b) % getPrime c /\
-    as_nat c h1 out == toDomain #c ((fromDomain #c (as_nat c h0 a) - fromDomain #c (as_nat c h0 b)) % getPrime c)))    
+    as_nat c h1 out == toDomain #c ((fromDomain #c (as_nat c h0 a) - fromDomain #c (as_nat c h0 b)) % getPrime c)))
 
 
-val mul: #c: curve -> f: felem c -> r: felem c -> out: widefelem c -> 
+val mul: #c: curve -> f: felem c -> r: felem c -> out: widefelem c ->
   Stack unit
     (requires fun h -> live h out /\ live h f /\ live h r /\ disjoint r out)
-    (ensures  fun h0 _ h1 -> modifies (loc out) h0 h1 /\ 
+    (ensures  fun h0 _ h1 -> modifies (loc out) h0 h1 /\
       wide_as_nat c h1 out = as_nat c h0 r * as_nat c h0 f)
 
 val isZero_uint64_CT: #c: curve ->  f: felem c -> Stack uint64
   (requires fun h -> live h f)
-  (ensures fun h0 r h1 -> modifies0 h0 h1 /\ 
+  (ensures fun h0 r h1 -> modifies0 h0 h1 /\
     (if as_nat c h0 f = 0 then uint_v r == pow2 64 - 1 else uint_v r == 0))
-    
+
 val compare_felem: #c: curve -> a: felem c -> b: felem c -> Stack uint64
-  (requires fun h -> live h a /\ live h b) 
-  (ensures fun h0 r h1 -> modifies0 h0 h1 /\ 
+  (requires fun h -> live h a /\ live h b)
+  (ensures fun h0 r h1 -> modifies0 h0 h1 /\
     (if as_nat c h0 a = as_nat c h0 b then uint_v r == pow2 64 - 1 else uint_v r = 0))
 
-val shiftLeftWord: #c: curve -> i: felem c -> o: lbuffer uint64 (getCoordinateLenU64 c *. 2ul)-> 
-  Stack unit 
+val shiftLeftWord: #c: curve -> i: felem c -> o: lbuffer uint64 (getCoordinateLenU64 c *. 2ul)->
+  Stack unit
     (requires fun h -> live h i /\ live h o /\ disjoint i o)
     (ensures fun h0 _ h1 -> modifies1 o h0 h1 /\ wide_as_nat c h1 o == as_nat c h0 i * (pow2 (getPower c)))
 
 
 inline_for_extraction noextract
-val mod64: #c: curve -> a: widefelem c -> Stack uint64 
-  (requires fun h -> live h a) 
+val mod64: #c: curve -> a: widefelem c -> Stack uint64
+  (requires fun h -> live h a)
   (ensures fun h0 r h1 -> modifies0 h0 h1 /\ wide_as_nat c h1 a % pow2 64 = uint_v r)
 
 
-val shift1_with_carry: #c: curve -> t: widefelem c -> t1: widefelem c -> carry: uint64 -> 
-  Stack unit 
+val shift1_with_carry: #c: curve -> t: widefelem c -> t1: widefelem c -> carry: uint64 ->
+  Stack unit
   (requires fun h -> live h t /\ live h t1 /\ disjoint t t1)
-  (ensures fun h0 _ h1 -> modifies (loc t1) h0 h1 /\ 
+  (ensures fun h0 _ h1 -> modifies (loc t1) h0 h1 /\
     (wide_as_nat c h0 t + pow2 (getLongPower c) * v carry) / pow2 64 = wide_as_nat c h1 t1)
 
 
-inline_for_extraction noextract 
+inline_for_extraction noextract
 val upload_one_montg_form: #c: curve -> b: felem c -> Stack unit
   (requires fun h -> live h b /\ as_nat c h b = 0)
   (ensures fun h0 _ h1 -> modifies (loc b) h0 h1 /\ as_nat c h1 b = toDomain #c 1)
@@ -194,15 +197,17 @@ val scalar_bit: #c: curve -> #buf_type: buftype
   -> n:size_t{v n < v (getScalarLen c)}
   -> Stack uint64
   (requires fun h0 -> live h0 s)
-  (ensures  fun h0 r h1 -> h0 == h1 /\ r == Spec.ECDSA.ith_bit_felem #c (as_seq h0 s) (v n) /\ 
+  (ensures  fun h0 r h1 -> h0 == h1 /\ r == Spec.ECDSA.ith_bit_felem #c (as_seq h0 s) (v n) /\
     v r <= 1)
 
 
-val mul_atomic: x: uint64 -> y: uint64 -> result: lbuffer uint64 (size 1) 
+val mul_atomic: x: uint64 -> y: uint64 -> result: lbuffer uint64 (size 1)
   -> temp: lbuffer uint64 (size 1) ->
   Stack unit
   (requires fun h -> live h result /\ live h temp /\ disjoint result temp)
   (ensures fun h0 _ h1 -> modifies (loc result |+| loc temp) h0 h1 /\ (
-    let h0 = Seq.index (as_seq h1 temp) 0 in 
-    let result = Seq.index (as_seq h1 result) 0 in 
+    let h0 = Seq.index (as_seq h1 temp) 0 in
+    let result = Seq.index (as_seq h1 result) 0 in
     uint_v result + uint_v h0 * pow2 64 = uint_v x * uint_v y))
+
+
